messageInvariantPrototypes/clientServer/automate/applicationProof.dfy
@@ -1,0 +1,116 @@
+include "messageInvariantsAutogen.dfy"
+
+module ClientServerProof {
+import opened Types
+import opened UtilitiesLibrary
+import opened DistributedSystem
+import opened MessageInvariants
+import opened Obligations
+
+
+/***************************************************************************************
+*                                Application Invariants                                *
+***************************************************************************************/
+
+ghost predicate ClientRequestsMonotonic(c: Constants, v: Variables)
+  requires v.WF(c)
+{
+  forall i, j, idx:nat |
+    && v.ValidHistoryIdx(i)
+    && v.ValidHistoryIdx(j)
+    && i <= j
+    && c.ValidClientIdx(idx) 
+  :: 
+    && v.History(i).clients[idx].requests <= 
+        v.History(j).clients[idx].requests
+}
+
+ghost predicate MonotonicityInv(c: Constants, v: Variables)
+  requires v.WF(c)
+{
+  ClientRequestsMonotonic(c, v)
+}
+
+
+// The server's requests must have come from sender client
+ghost predicate ServerRequestsValid(c: Constants, v: Variables)
+  requires v.WF(c)
+{
+  forall i| 
+    && v.ValidHistoryIdx(i)
+    && v.History(i).GetServer(c).currentRequest.Some?
+  ::
+    && var req := v.History(i).GetServer(c).currentRequest.value;
+    && c.ValidClientIdx(req.clientId)
+    && req.reqId in v.History(i).clients[req.clientId].requests
+}
+
+ghost predicate ApplicationInv(c: Constants, v: Variables)
+  requires v.WF(c)
+{
+  ServerRequestsValid(c, v)
+}
+
+ghost predicate Inv(c: Constants, v: Variables)
+{
+  && v.WF(c)
+  && MessageInv(c, v)
+  && MonotonicityInv(c, v)
+  && ApplicationInv(c, v)
+  && Safety(c, v)
+}
+
+lemma InvImpliesSafety(c: Constants, v: Variables)
+  requires Inv(c, v)
+  ensures Safety(c, v)
+{}
+
+lemma InitImpliesInv(c: Constants, v: Variables)
+  requires Init(c, v)
+  ensures Inv(c, v)
+{
+  InitImpliesMessageInv(c, v);
+}
+
+lemma InvInductive(c: Constants, v: Variables, v': Variables)
+  requires Inv(c, v)
+  requires Next(c, v, v')
+  ensures Inv(c, v')
+{
+  VariableNextProperties(c, v, v');
+  MessageInvInductive(c, v, v');
+  InvNextClientRequestsMonotonic(c, v, v');
+  InvNextServerRequestsValid(c, v, v');
+}
+
+/***************************************************************************************
+*                                        Proof                                         *
+***************************************************************************************/
+
+lemma InvNextClientRequestsMonotonic(c: Constants, v: Variables, v': Variables)
+  requires v.WF(c)
+  requires ClientRequestsMonotonic(c, v)
+  requires Next(c, v, v')
+  ensures ClientRequestsMonotonic(c, v')
+{
+  VariableNextProperties(c, v, v');
+}
+
+lemma InvNextServerRequestsValid(c: Constants, v: Variables, v': Variables)
+  requires Inv(c, v)
+  requires Next(c, v, v')
+  ensures ServerRequestsValid(c, v')
+{
+  VariableNextProperties(c, v, v');
+  forall i| 
+    && v'.ValidHistoryIdx(i)
+    && v'.History(i).GetServer(c).currentRequest.Some?
+  ensures
+    && var req := v'.History(i).GetServer(c).currentRequest.value;
+    && c.ValidClientIdx(req.clientId)
+    && req.reqId in v'.History(i).clients[req.clientId].requests
+  {}
+}
+
+}  // end module ClientServerProof
+
