messageInvariantPrototypes/clientServer/types.dfy
@@ -9,6 +9,11 @@ module Types {
 
   datatype Message =
     RequestMsg(r: Request) | ResponseMsg(r: Request)
+  {
+    ghost function Src() : nat {
+      if this.RequestMsg? then r.clientId else 0
+    }
+  }
 
   datatype MessageOps = MessageOps(recv:Option<Message>, send:Option<Message>)
 } // end module Types
